# Solution to exercise 1.1

This is a literate Rzk file:

```rzk
#lang rzk-1
```

## Problem statement

!!! question "Exercise 1.1"
    Given functions $f : A \to B$ and $g : B \to C$,
    define their composite $g \circ f : A \to C$.
    Show that we have $h \circ (g \circ f) \equiv (h \circ g) \circ f$.

## Solution

First, the definition of the composition operation is provided as:

$$
g \circ f :\equiv \lambda (x: A) . g(f(x))
$$

Then, associativity can be demonstrated by evaluating both sides of the equality and reaching the same result:

$$
    \begin{align*}
        h \circ (g \circ f) & \equiv \lambda x. h((g\circ f)(x)) \\
                            & \equiv \lambda x. h((\lambda x' . g(f(x'))) (x)) \\
                            & \equiv \lambda x. h(g(f(x)))
    \end{align*}
$$

$$
    \begin{align*}
        (h \circ g) \circ f & \equiv \lambda x. (h\circ g)(f(x)) \\
                            & \equiv \lambda x. (\lambda y . h(g(y)))(f(x)) \\
                            & \equiv \lambda x. h(g(f(x)))
    \end{align*}
$$

This can be represented in rzk like so:

```rzk
#define compose
  ( A B C : U)
  ( g : B → C)
  ( f : A → B)
  : A → C
  := \ x → g (f x)
```

Associativity is automatic (by `refl`):

```rzk
#define composition-associativity
  ( A B C D : U)
  ( f : A → B)
  ( g : B → C)
  ( h : C → D)
  : compose A C D h (compose A B C g f) = compose A B D (compose B C D h g) f
  := refl
```

An explicit proof (not checked by `rzk`):

```
compose A C D h (compose A B C g f)
= \ x → h ((compose A B C g f) x)       (unfolding compose)
= \ x → h ((\ x2 → g (f x2)) x)         (unfolding compose)
= \ x → h (g (f x))                     (beta reduction)
= \ x → (\ x2 → h (g x2)) (f x)         (beta reduction)
= \ x → (compose B C D h g) (f x)       (fold compose)
= compose A B D (compose B C D h g) f   (fold compose)
```
